examples/Row.v
@@ -1,0 +1,88 @@
+Require Import FreeSpec.Interface.
+Require Import FreeSpec.Control.
+Require Import FreeSpec.Program.
+Require Import FreeSpec.Semantics.
+Require Import FreeSpec.Row.
+Require Import Coq.Lists.List.
+
+Local Open Scope free_control_scope.
+Local Open Scope free_row_scope.
+
+Inductive NatStack
+  : Type -> Type :=
+| Push (x: nat)
+  : NatStack unit
+| Pop
+  : NatStack nat.
+
+Definition push_nat
+           {eff:  list (Type -> Type)} `{HasEffect eff NatStack}
+           (x:    nat)
+  : Program (row eff) unit :=
+  inj_effect (Push x).
+
+Definition pop_nat
+           {eff:  list (Type -> Type)} `{HasEffect eff NatStack}
+  : Program (row eff) nat :=
+  inj_effect Pop.
+
+Inductive LogNat
+  : Type -> Type :=
+| Log (x:  nat)
+  : LogNat unit.
+
+Definition log_nat
+           {eff:  list (Type -> Type)} `{HasEffect eff LogNat}
+           (n:    nat)
+  : Program (row eff) unit :=
+  inj_effect (Log n).
+
+Definition my_program
+           {eff:  list (Type -> Type)} `{HasEffect eff NatStack}
+           `{HasEffect eff LogNat}
+           (x:    nat)
+  : Program (row eff) unit :=
+  y <- pop_nat;
+    push_nat x;;
+             log_nat y.
+
+Definition stack_sem
+  : Semantics NatStack :=
+  mkSemantics (fun (A:  Type)
+                   (l:  list nat)
+                   (e:  NatStack A)
+               => match e with
+                  | Push x
+                    => (tt, x :: l)
+                  | Pop
+                    => match l with
+                       | x :: r
+                         => (x, r)
+                       | _
+                         => (0, nil)
+                       end
+                  end) nil.
+
+Definition log_sem
+  : Semantics LogNat :=
+  mkSemantics (fun (A:  Type)
+                   (l:  list nat)
+                   (e:  LogNat A)
+               => match e with
+                  | Log x
+                    => (tt, x :: l)
+                  end) nil.
+
+Definition example_semantics :=
+  <| stack_sem; log_sem |>.
+
+Definition test :=
+  evalProgram example_semantics (my_program 0).
+
+Goal (test = tt).
+  remember (runProgram example_semantics pop_nat).
+  cbn in Heqp.
+  unfold push_sem in Heqp;
+    unfold sem_nil in Heqp.
+  reflexivity.
+Qed.
